<?xml version="1.0" encoding="UTF-8"?>

<section xml:id="sec-antidifferentiation-rules" xmlns:xi="http://www.w3.org/2001/XInclude">
  <title>Antidifferentiation Rules</title>

  <p>
    The process of finding an antiderivative is called <em>antidifferentiation</em>.
    Up to this point, we've antidifferentiated by recalling differentiation rules.
    We now observe some general rules for antidifferentiation.
  </p>
  
  <exercise xml:id="exc-power-rule">
    <title>Discovering the Power Rule</title>
    
    <instructions>
      Find the given indefinite integral.  Do you see a pattern?
    </instructions>

    <task>
      <statement>
        <p>
          <m>\dsp\int x\,dx</m>
        </p>
      </statement>

      <answer>
        <p>
          <m>\dsp\int x\,dx=\tfrac{x^2}{2}+C</m>
        </p>
      </answer>
    </task>

    <task>
      <statement>
        <p>
          <m>\dsp\int x^2\,dx</m>
        </p>
      </statement>

      <answer>
        <p>
          <m>\dsp\int x^2\,dx=\tfrac{x^3}{3}+C</m>
        </p>
      </answer>
    </task>

    <task>
      <statement>
        <p>
          <m>\dsp\int x^3\,dx</m>
        </p>
      </statement>

      <answer>
        <p>
          <m>\dsp\int x^3\,dx=\tfrac{x^4}{4}+C</m>
        </p>
      </answer>
    </task>

    <task>
      <statement>
        <p>
          <m>\dsp\int x^n\,dx</m>, where <m>n\neq -1</m> is a constant
        </p>
      </statement>

      <answer>
        <p>
          <m>\dsp\int x^n\,dx=\tfrac{x^{n+1}}{n+1}+C</m>
        </p>
      </answer>

      <solution>
        <p>
          Based on our answers above, we guess that
          <me>
            \dsp\int x^n\,dx=\tfrac{x^{n+1}}{n+1}+C.
          </me>
          We can check that our guess is correct by differentiating:
          <me>
            \tfrac{d}{dx}\left[\tfrac{x^{n+1}}{n+1}\right]=x^n.
          </me>
        </p>    
      </solution>
    </task>
  </exercise>

  <p>
    The rule that you picked up on in <xref ref="exc-power-rule"/> is called the <em>Power Rule</em>.  
    In words, the Power Rule says that to antidifferentiate <m>f(x)=x^n</m>, we add one to the exponent, and divide by the new exponent.
    So far, we've only used the Power Rule in the case that <m>n</m> is a positive integer, but it works for all real numbers <m>n\neq -1</m>.
  </p>

  <exercise>

    <title>Using the Power Rule</title>
    
    <instructions>
      Find the given indefinite integral.
    </instructions>

    <task>
      <statement>
        <p>
          <m>\dsp\int x^{5}\,dx</m>
        </p>
      </statement>

      <answer>
        <p>
          <m>\dsp\int x^{5}\,dx=\tfrac{x^6}{6}+C</m>
        </p>
      </answer>
    </task>

    <task>
      <statement>
        <p>
          <m>\dsp\int \tfrac{1}{x^2}\,dx</m>
        </p>
      </statement>

      <answer>
        <p>
          <m>\dsp\int \tfrac{1}{x^2}\,dx=-\tfrac{1}{x}+C</m>
        </p>
      </answer>

      <solution>
        <p>
          Recall that <m>\frac{1}{x^2}=x^{-2}</m>, so we have
          <me>
            \dsp\int \tfrac{1}{x^2}\,dx=\dsp\int x^{-2}\,dx=\tfrac{x^{-1}}{-1}+C=-\tfrac{1}{x}+C.
          </me>
          When applying the Power Rule, remember that we always <em>add one</em> to the exponent, and then divide by the new exponent.
        </p>
      </solution>
    </task>

    <task>
      <statement>
        <p>
          <m>\dsp\int \sqrt{x}\,dx</m>
        </p>
      </statement>

      <answer>
        <p>
          <m>\dsp\int \sqrt{x}\,dx=\tfrac{2}{3}x^{3/2}+C</m>
        </p>
      </answer>

      <solution>
        <p>
          Recall that <m>\sqrt{x}=x^{\tfrac{1}{2}}</m>, so we have
          <me>
            \dsp\int \sqrt{x}\,dx=\frac{x^{\tfrac{1}{2}}}{\tfrac{3}{2}}+C=\tfrac{2}{3}x^{\tfrac{3}{2}}+C
          </me>
        </p>
      </solution>
    </task>

    <task>
      <statement>
        <p>
          <m>\dsp\int \tfrac{1}{\sqrt{x}}\,dx</m>
        </p>
      </statement>

      <answer>
        <p>
          <m>\dsp\int \tfrac{1}{\sqrt{x}}\,dx=2\sqrt{x}+C</m>
        </p>
      </answer>

      <solution>
        <p>
          We can write <m>\tfrac{1}{\sqrt{x}}=x^{-\frac{1}{2}}</m>, so we have
          <me>
            \dsp\int \tfrac{1}{\sqrt{x}}\,dx=\int x^{-\frac{1}{2}}\,dx=\frac{x^{\frac{1}{2}}}{\frac{1}{2}}+C=2\sqrt{x}+C.
          </me>
        </p>
      </solution>
    </task>
    

  </exercise>

  <exercise>
    <title>When The Power Rule Fails</title>

    <task>
      <statement>
        <p>
          Can the Power Rule be used to find <m>\dsp\int\tfrac{1}{x}\,dx</m>?
        </p>
      </statement>

      <answer>
        <p>
          No.
        </p>
      </answer>

      <solution>
        <p>
          Recall that <m>\frac{1}{x}=x^{-1}</m>.  
          If we tried to apply the Power Rule, we would have to divide by zero!  
          <!-- So we cannot use the Power Rule to find <m>\dsp\int\tfrac{1}{x}\,dx</m>. -->
        </p>
      </solution>
    </task>

    <task>
      <statement>
        <p>
          Find <m>\dsp\int \tfrac{1}{x}\,dx</m>.
        </p>
      </statement>

      <hint>
        <p>
          Can you think of a function whose derivative is <m>\tfrac{1}{x}</m>?
        </p>
      </hint>

      <answer>
        <p>
          <m>\dsp\int \tfrac{1}{x}\,dx=\ln|x|+C</m>,
          where <m>|x|</m> denotes the <em>absolute value</em> of <m>x</m>.
        </p>

        <p>
          <b>Note:</b> Your first guess might have been that <m>\int \tfrac{1}{x}\,dx=\ln(x)+C</m>, without the absolute value.
          The minor issue with this guess is that <m>\ln(x)</m> is defined only for <m>x>0</m>, while <m>\frac{1}{x}</m> is defined for all <m>x\neq 0</m>.
          Observe that <m>\ln|x|</m> is defined for all <m>x\neq 0</m>, 
          and in fact one can show that <m>\frac{d}{dx}\left[\ln|x|\right]=\frac{1}{x}</m> for all <m>x\neq 0</m>; see the solutions below.
        </p>
      </answer>

      <solution>
        <p>
          We will show that <m>\tfrac{d}{dx}\left[\ln|x|\right]=\frac{1}{x}</m> for all <m>x\neq 0</m>, which means that
          <me>
            \dsp\int \tfrac{1}{x}\,dx=\ln|x|+C.
          </me>
          Recall that <m>|x|</m> is defined by
          <me>
            |x|=
            \begin{cases}
              x, &amp; \text{ if } x\geq 0\text{;}\\
              -x, &amp; \text{ if } x&lt; 0\text{.}
            \end{cases}
          </me>
          So if <m>x>0</m>, then we have <m>|x|=x</m>, hence
          <me>
            \tfrac{d}{dx}\left[\ln|x|\right]=\tfrac{d}{dx}\left[\ln(x)\right]=\tfrac{1}{x}.
          </me>
          On the other hand, if <m>x&lt; 0</m>, then we have <m>|x|=-x</m>, hence
          <md>
            <mrow>
              \tfrac{d}{dx}\left[\ln|x|\right]\amp =\tfrac{d}{dx}\left[\ln(-x)\right]
            </mrow>
            <mrow>
              \amp=\tfrac{1}{-x}\cdot -1 \hspace{1cm} \text{(by the Chain Rule)}
            </mrow>
            <mrow> 
              \amp=\tfrac{1}{x}. 
            </mrow>  
          </md>
          So for all <m>x\neq 0</m>, we have <m>\tfrac{d}{dx}\left[\ln|x|\right]=\frac{1}{x}</m>, as desired.
        </p>
      </solution>

    </task>

  </exercise>

  <p>
    To verify an antidifferentiation rule of the form
    <m>
      \int f(x)\,dx=F(x)+C,
    </m>
    we simply need to check that <m>F'(x)=f(x)</m> for all <m>x</m> in the domain of <m>f</m>.
    All of the antidifferentiation rules stated in the next theorem can be verified in this manner.
  </p>

  <theorem xml:id="thm-basic-antidifferentiation-rules">

    <title>Basic Antidifferentiation Rules</title>
    <statement>
      <p>
        <ol>
          <li xml:id="basic-rule-const">
            <p>
              <m>
                \dsp\int a\,dx=ax+C
              </m>, where <m>a</m> is a constant
            </p>
          </li>
          <li xml:id="basic-rule-power">
            <p>
              <m>
                \dsp\int x^n\,dx=\frac{x^{n+1}}{n+1}+C
              </m>, where <m>n\neq -1</m> is a constant
            </p>
          </li>
          <li xml:id="basic-rule-ln">
            <p>
              <m>
                \dsp\int \frac{1}{x}\,dx=\ln|x|+C
              </m>
            </p>
          </li>
          <li xml:id="basic-rule-exp">
            <p>
              <m>
                \dsp\int e^x\,dx=e^x+C
              </m>
            </p>
          </li>
          <li xml:id="basic-rule-expb">
            <p>
              <m>
                \dsp\int b^x\,dx=\frac{b^x}{\ln(b)}+C
              </m>, where <m>b\neq 1</m> is a positive constant 
            </p>
          </li>
          <li xml:id="basic-rule-cos">
            <p>
              <m>
                \dsp\int\cos(\theta)\,d\theta=\sin(\theta)+C
              </m>
            </p>
          </li>
          <li xml:id="basic-rule-sin">
            <p>
              <m>
                \dsp\int \sin(\theta)\,d\theta=-\cos(\theta)+C
              </m>
            </p>
          </li>
          <li xml:id="basic-rule-sec2">
            <p>
              <m>
                \dsp\int\sec^2(\theta)\,d\theta=\tan(\theta)+C
              </m>
            </p>
          </li>
          <li xml:id="basic-rule-csc2">
            <p>
              <m>
                \dsp\int\csc^2(\theta)\,d\theta=-\cot(\theta)+C
              </m>
            </p>
          </li>
          <li xml:id="basic-rule-sectan">
            <p>
              <m>
                \dsp\int\sec(\theta)\tan(\theta)\,d\theta=\sec(\theta)+C
              </m>
            </p>
          </li>
          <li xml:id="basic-rule-csccot">
            <p>
              <m>
                \dsp\int\csc(\theta)\cot(\theta)\,d\theta=-\csc(\theta)+C
              </m>
            </p>
          </li>
          <!-- <li xml:id="basic-rule-tan">
            <p>
              <m>
                \dsp\int\tan(\theta)\,d\theta=\ln|\sec(\theta)|+C
              </m>
            </p>
          </li>
          <li xml:id="basic-rule-cot">
            <p>
              <m>
                \dsp\int\cot(\theta)\,d\theta=\ln|\sin(\theta)|+C
              </m>
            </p>
          </li>
          <li xml:id="basic-rule-sec">
            <p>
              <m>
                \dsp\int \sec(\theta)\,d\theta=\ln|\sec(\theta)+\tan(\theta)|+C
              </m>
            </p>
          </li>
          <li xml:id="basic-rule-csc">
            <p>
              <m>
                \dsp\int\csc(\theta)\,d\theta=\ln|\csc(\theta)-\cot(\theta)|+C
              </m>
            </p>
          </li> -->
          <li xml:id="basic-rule-arctan">
            <p>
              <m>
                \dsp\int\frac{1}{1+x^2}\,dx=\arctan(x)+C
              </m>
            </p>
          </li>
          <li xml:id="basic-rule-arcsin">
            <p>
              <m>
                \dsp\int\frac{1}{\sqrt{1-x^2}}\,dx=\arcsin(x)+C
              </m>
            </p>
          </li>
          <li xml:id="basic-rule-arcsec">
            <p>
              <m>
                \dsp\int \frac{1}{x\sqrt{x^2-1}}\,dx=\arcsec(x)+C
              </m>
            </p>
          </li>
        </ol>
      </p> 
    </statement>

  </theorem>

  <p>
    We used the variables <m>x</m> and <m>\theta</m> to state our basic antidifferentiation rules, but the rules hold for any variable.  
    Remember that the differential specifies the variable of antidifferentiation.  
    So for example, using <xref ref="basic-rule-const" text="local">Basic Rule</xref>, we have
    <me>
      \int 5\,dx=5x+C
    </me>
    and
    <me>
      \int 5\,du=5u+C.
    </me>
    
  </p>

  <exercise>
    <title>
      Using basic antidifferentiation rules
    </title>

    <instructions>
      Find the given indefinite integral.
    </instructions>
    
    <task>
      <statement>
        <p>
          <m>\dsp\int\frac{1}{1+u^2}\,du</m>
        </p>
      </statement>

      <answer>
        <p>
          <m>\dsp\int\frac{1}{1+u^2}\,du=\arctan(u)+C</m>, by <xref ref="basic-rule-arctan" text="local">Basic Rule</xref>
        </p>
      </answer>
    </task>

    <task>
      <statement>
        <p>
          <m>\dsp\int\sec(x)\tan(x)\,dx</m>
        </p>
      </statement>

      <answer>
        <p>
          <m>\dsp\int\sec(x)\tan(x)\,dx=\sec(x)+C</m>, by <xref ref="basic-rule-sectan" text="local">Basic Rule</xref>
        </p>
      </answer>
    </task>

    <task>
      <statement>
        <p>
          <m>\dsp\int\pi\,dx</m>
        </p>
      </statement>

      <answer>
        <p>
          <m>\dsp\int\pi\,dx=\pi x+C</m>, by <xref ref="basic-rule-const" text="local">Basic Rule</xref>
        </p>
      </answer>
    </task>
    
  </exercise>

  <p>
    Now we derive some antidifferentiation rules for functions that are built up from simpler functions.  
    Remember that we did the same for differentiation rules in Calculus 1, with the Constant Multiple, Sum, Difference, Product, Quotient, and Chain Rules.
    We start with the Constant Multiple Rule, Sum, and Difference Rules for antidifferentiation.
  </p>

  <theorem xml:id="thm-constant-multiple-rule">

    <title>The Constant Multiple Rule</title>
    
    <statement>
      <p>
        Let <m>f</m> be a function with antiderivative <m>F</m>, and let <m>a</m> be a constant.  Then
        <me>
          \int a f(x)\,dx= aF(x)+C.
        </me>
        Alternatively, we can write
        <men xml:id="constant-multiple-rule">
          \int a f(x)\,dx=a\int f(x)\,dx.
        </men>
      </p>
    </statement>
  </theorem>

  <proof>
    <p>
      Since <m>F</m> is an antiderivative of <m>f</m>, we have <m>\tfrac{d}{dx}\left[F(x)\right]=f(x)</m>.  
      Hence, by the Constant Multiple Rule for differentiation, we have 
      <me>
        \tfrac{d}{dx}\left[aF(x)\right]=a\tfrac{d}{dx}\left[F(x)\right]=af(x).
      </me>
      Therefore, we conclude that <m>\dsp\int a f(x)\,dx= aF(x)+C</m>.
    </p>
  </proof>

  <theorem xml:id="thm-sum-rule">

    <title>The Sum Rule</title>
    
    <statement>
      <p>
        Let <m>f</m> and <m>g</m> be functions with antiderivatives <m>F</m> and <m>G</m>, respectively.  Then
        <me>
          \int f(x)+ g(x)\,dx= F(x)+G(x)+C.
        </me>
        Alternatively, we can write
        <men xml:id="sum-rule">
          \int f(x)+ g(x)\,dx=\int f(x)\,dx+\int g(x)\,dx.
        </men>
      </p>
    </statement>
  </theorem>

  <proof>
    <p>
      Since <m>F</m> and <m>G</m> are antiderivatives of <m>f</m> and <m>g</m>, respectively, we have <m>\tfrac{d}{dx}\left[F(x)\right]=f(x)</m> and <m>\tfrac{d}{dx}\left[G(x)\right]=g(x)</m>.  
      Hence, by the Sum Rule for differentiation, we have 
      <me>
        \tfrac{d}{dx}\left[F(x)+G(x)\right]=\tfrac{d}{dx}\left[F(x)\right]+\tfrac{d}{dx}\left[G(x)\right]=f(x)+g(x).
      </me>
      Therefore, we conclude that <m>\dsp\int f(x)+g(x)\,dx= F(x)+G(x)+C</m>.
    </p>
  </proof>

  <p>
    Together, the Sum Rule and the Constant Multiple Rule (with the constant <m>-1</m>) give us the <em>Difference Rule</em>:
    <men xml:id="difference-rule">
      \int f(x)-g(x)\,dx=\int f(x)\,dx-\int g(x)\,dx.
    </men>
  </p>

  <exercise>

    <title>Using the Constant Multiple, Sum, and Difference Rules</title>

    <instructions>
      Find the given indefinite integral.
    </instructions>

    <task>
      <statement>
        <p>
          <m>
            \dsp\int \cos(\theta)+\sin(\theta)\,d\theta
          </m>
        </p>
      </statement>

      <answer>
        <p>
          <m>\dsp\int \cos(\theta)+\sin(\theta)\,d\theta=\sin(\theta)-\cos(\theta)+C</m>
        </p>
      </answer>

      <solution>
        <p>
          By the <xref ref="sum-rule" text="custom">Sum Rule</xref>, <xref ref="basic-rule-cos" text="local">Basic Rule</xref>, and <xref ref="basic-rule-sin" text="local">Basic Rule</xref> we have
          <md>
            <mrow>\int \cos(\theta)+\sin(\theta)\,d\theta\amp=\int\cos(\theta)\,d\theta+\int\sin(\theta)\,d\theta</mrow>
            <mrow>\amp=\sin(\theta)-\cos(\theta)+C.</mrow>
          </md>
          Notice that even though we had two indefinite integrals on the right-hand-side, we write just one constant of integration <m>C</m>.
          One can think of <m>C</m> as the sum of two separate constants of integration <m>C_1</m> and <m>C_2</m>.
        </p>
      </solution>
    </task>

    <task>
      <statement>
        <p>
          <m>
            \dsp\int 4u^2\,du
          </m>
        </p>
      </statement>

      <answer>
        <p>
          <m>\dsp\int 4u^2\,du=\frac{4}{3}u^3+C</m>
        </p>
      </answer>

      <solution>
        <p>
          By the <xref ref="constant-multiple-rule" text="custom">Constant Multiple Rule</xref> and <xref ref="basic-rule-power" text="local">Basic Rule</xref>, we have
          <me>
            \int 4u^2\,du=4\int u^2\,du=4\cdot \frac{u^3}{3}+C=\frac{4}{3}u^3+C.
          </me>
          Notice again that we use the simple constant of integration <m>C</m>.
          One can think of <m>C</m> as <m>4C_1</m>, where <m>C_1</m> is the constant of integration from <m>\int u^2\,du</m>.
        </p>
      </solution>
    </task>

    <task>
      <statement>
        <p>
          <m>
            \dsp\int 2e^x-6x\,dx
          </m>
        </p>
      </statement>

      <answer>
        <p>
          <m>\dsp\int 2e^x-6x\,dx=2e^x-3x^2+C</m>
        </p>
      </answer>

      <solution>
        <p>
          <md>
            <mrow> \int 2e^x-6x\,dx \amp = \int 2e^x\,dx-\int 6x\,dx \amp \text{by the }<xref ref="difference-rule" text="custom">Difference Rule</xref>\amp</mrow>
            <mrow> \amp = 2\int e^x\,dx-6\int x\,dx \amp \text{by the }<xref ref="constant-multiple-rule" text="custom">Constant Multiple Rule</xref>\amp</mrow>
            <mrow> \amp = 2e^x-3x^2+C \amp \text{by Basic Rules }<xref ref="basic-rule-power" text="local"></xref>\text{ and }<xref ref="basic-rule-exp" text="local"></xref>\amp</mrow>
          </md>
        </p>
      </solution>
    </task>

    <task>
      <statement>
        <p>
          <m>
            \dsp\int \sec(\theta)\left(\sec(\theta)+\tan(\theta)\right)\,d\theta
          </m>
        </p>
      </statement>

      <answer>
        <p>
          <m>\dsp\int \sec(\theta)\left(\sec(\theta)+\tan(\theta)\right)\,d\theta=\tan(\theta)+\sec(\theta)+C</m>
        </p>
      </answer>

      <solution>
        <p>
          We first apply the distributive law, so that we can use our rules for antidifferentiation:
          <md>
            <mrow> \amp \int  \sec(\theta)\left(\sec(\theta)+\tan(\theta)\right)\,d\theta </mrow>
            <mrow> \amp = \int \sec^2(\theta)+\sec(\theta)\tan(\theta)\,d\theta \amp \text{by algebra}\amp</mrow>
            <mrow> \amp = \int\sec^2(\theta)\,d\theta+\int\sec(\theta)\tan(\theta)\,d\theta \amp \text{by the }<xref ref="sum-rule" text="custom">Sum Rule</xref>\amp</mrow>
            <mrow> \amp = \tan(\theta)+\sec(\theta)+C \amp \text{by Basic Rules }<xref ref="basic-rule-sec2" text="local"></xref>\text{ and }<xref ref="basic-rule-sectan" text="local"></xref>\amp</mrow>
          </md>
        </p>
      </solution>
    </task>

    <task>
      <statement>
        <p>
          <m>
            \dsp\int \frac{x^3-2x+1}{x}\,dx
          </m>
        </p>
      </statement>

      <answer>
        <p>
          <m>\dsp\int \frac{x^3-2x+1}{x}\,dx=\frac{1}{3}x^3-2x+\ln|x|+C</m>
        </p>
      </answer>

      <solution>
        <p>
          We first divide through by <m>x</m>, so that we can use our rules for antidifferentiation:
          <md>
            <mrow> \int \frac{x^3-2x+1}{x}\,dx\amp = \int x^2-2+\frac{1}{x}\,dx</mrow>
            <mrow> \amp = \int x^2\,dx-\int 2\,dx+\int\frac{1}{x}\,dx </mrow>
            <mrow> \amp = \frac{1}{3}x^3-2x+\ln|x|+C</mrow>
          </md>
        </p>
      </solution>
    </task>


  </exercise>
  
  

</section>

